\documentclass{article}

% Packages
\usepackage[a4paper]{geometry}
\usepackage[utf8]{inputenc}
\usepackage{amsmath}
\usepackage{progproving}
\usepackage{listings}

\geometry{top=25mm,bottom=25mm,inner=25mm,outer=20mm}
\allowdisplaybreaks

\begin{document}
\title{ProgProving package : Example}

\author{BERG Lucas}

\maketitle

\section{Introduction}
    This document is an example for the ProgProving package. We will prove the following function:

    \begin{lstlisting}[language=C]
int sum(int array[], int length) {
    int total = 0;
    int i = 0;
    while (i < length) {
        total = total + array[i];
        i = i + 1;
    }
    return total;
}
    \end{lstlisting}

\section{Specifications}
    First, let's write the specifications of the function.
    
    \subsection{Header}
        \begin{lstlisting}[language=C]
int sum(int array[], int length)
        \end{lstlisting}
    
    \subsection{Environment}
        /
    
    \subsection{Precondition}
        \begin{flalign*}
            & \pre = \state{
                & 0 \leq length \wedge \\
                & length = \text{size of array[]}
            } &
        \end{flalign*}
    
    \subsection{Postcondition}
        \begin{flalign*}
            & \post = \state{
                & 0 \leq length \wedge \\
                & length = \text{size of array[]} \wedge \\
                & sum = \sum^{length-1}_{j=0} array[j] \wedge \\
                & length = length_0 \wedge \\
                & array = array_0
            } &
        \end{flalign*}

        with:
        \begin{itemize}
            \item $length_0$ which is the value of $length$ before the function call
            \item $array_0$ which is the value of $array$ before the function call
        \end{itemize}

\section{Proof using the strongest postcondition (sp)}
    \subsection{Definitions}
        \begin{flalign*}
            & \init \equiv
                \seq{
                    & total := 0; \\
                    & i := 0;
                }
            & \\
            & \iter \equiv 
                \seq{
                    & total := total + array[i]; \\
                    & i := i + 1;
                }
            & \\
            & \term \equiv  sum := total;
        \end{flalign*}

    \subsection{The instructions before the loop}
        First, we need to calculate the instructions before the loop by doing $\state{\pre} \init \state{\lpre}$.

        \begin{flalign*}
            & \ppsp{\init}{\state{\pre}} & \\
        %
        %
        %
        =   & \ppsp{
                \seq{
                    & total := 0; \\
                    & i := 0;
                }
            }{
                \state{
                    & 0 \leq length \wedge \\
                    & length = \text{size of array[]}
                }
            } & \\
        %
        %
        %
        =   & \ppsp{
                i := 0;
            }{
                \state{
                    & 0 \leq length \wedge \\
                    & length = \text{size of array[]}
                }[total/total']
                \wedge
                \state{
                    total := 0
                }[total/total']
            } & \\
        %
        %
        %
        =   & \ppsp{
                i := 0;
            }{
                \state{
                    & 0 \leq length \wedge \\
                    & length = \text{size of array[]}
                }
                \wedge
                \state{
                    total = 0
                }
            } & \\
        %
        %
        %
        =   & \ppsp{
                i := 0;
            }{
                \state{
                    & 0 \leq length \wedge \\
                    & length = \text{size of array[]} \wedge \\
                    & total = 0
                }
            } & \\
        %
        %
        %
        =   & \state{
                & 0 \leq length \wedge \\
                & length = \text{size of array[]} \wedge \\
                & total = 0
            }[i/i']
            \wedge
            \state{
                i := 0
            }[i/i'] & \\
        %
        %
        %
        =   & \state{
                & 0 \leq length \wedge \\
                & length = \text{size of array[]} \wedge \\
                & total = 0
            }
            \wedge
            \state{
                i = 0
            } & \\
        %
        %
        %
        =   & \state{
                & 0 \leq length \wedge \\
                & length = \text{size of array[]} \wedge \\
                & total = 0 \wedge \\
                & i = 0
            } & \\
        %
        %
        %
        =   & \lpre &
        \end{flalign*}

        All right, we got the loop precondition so we can move on to the next step.
    
    \subsection{The loop instruction}

        Now, we need to prove the loop instruction. There are 4 steps.

        \subsubsection{Find the loop invariant $\inv$}
            First, we need to find the loop invariant $\inv$. In most cases, the invariant will describe the state of the loop using i-1. In our case, the invariant is:

            \begin{flalign*}
                & \inv = \state{
                    & 0 \leq i \leq length \wedge \\
                    & length = \text{size of array[]} \wedge \\
                    & total = \sum^{i-1}_{j = 0} array[j]
                } &
            \end{flalign*}
        
        \subsubsection{Proof that $\inv$ is an invariant}
            Now, we have to prove $\{ \inv \wedge \cond \} \iter \{ \inv \}$. If we can prove that, this means that the invariant is correct.
            First, let's define $\inv \wedge \cond$

            \begin{flalign*}
                & \inv \wedge \cond = \state{
                    & 0 \leq i \leq length \wedge \\
                    & length = \text{size of array[]} \wedge \\
                    & total = \sum^{i-1}_{j = 0} array[j]
                } \wedge \state{
                    i < length
                } = \state{
                    & 0 \leq i < length \wedge \\
                    & length = \text{size of array[]} \wedge \\
                    & total = \sum^{i-1}_{j = 0} array[j]
                } &
            \end{flalign*}

            Then, we can do a sp to check if $\inv$ is an invariant.

            \begin{flalign*}
                    & \ppsp{\iter}{\inv \wedge \cond} & \\
                %
                %
                %
                =   & \ppsp{
                        \seq{
                            & total := total + array[i]; \\
                            & i := i + 1;
                        }
                    }{
                        \state{
                            & 0 \leq i < length \wedge \\
                            & length = \text{size of array[]} \wedge \\
                            & total = \sum^{i-1}_{j = 0} array[j]
                        }
                    } & \\
                %
                %
                %
                =   & \ppsp{
                        i := i + 1;
                    }{
                        \state{
                            & 0 \leq i < length \wedge \\
                            & length = \text{size of array[]} \wedge \\
                            & total = \sum^{i-1}_{j = 0} array[j]
                        }[total/total']
                        \wedge
                        \state{
                            total := total + array[i]
                        }[total/total']
                    } & \\
                %
                %
                %
                =   & \ppsp{
                        i := i + 1;
                    }{
                        \state{
                            & 0 \leq i < length \wedge \\
                            & length = \text{size of array[]} \wedge \\
                            & total' = \sum^{i-1}_{j = 0} array[j]
                        }
                        \wedge
                        \state{
                            total = total' + array[i]
                        }
                    } & \\
                %
                %
                %
                =   & \ppsp{
                        i := i + 1;
                    }{
                        \state{
                            & 0 \leq i < length \wedge \\
                            & length = \text{size of array[]} \wedge \\
                            & total' = \sum^{i-1}_{j = 0} array[j]
                        }
                        \wedge
                        \state{
                            total - array[i] = total'
                        }
                    } & \\
                %
                %
                %
                =   & \ppsp{
                        i := i + 1;
                    }{
                        \state{
                            & 0 \leq i < length \wedge \\
                            & length = \text{size of array[]} \wedge \\
                            & total - array[i] = \sum^{i-1}_{j = 0} array[j]
                        }
                    } & \\
                %
                %
                %
                =   & \ppsp{
                        i := i + 1;
                    }{
                        \state{
                            & 0 \leq i < length \wedge \\
                            & length = \text{size of array[]} \wedge \\
                            & total = (\sum^{i-1}_{j = 0} array[j]) + array[i]
                        }
                    } & \\
                %
                %
                %
                =   & \ppsp{
                        i := i + 1;
                    }{
                        \state{
                            & 0 \leq i < length \wedge \\
                            & length = \text{size of array[]} \wedge \\
                            & total = \sum^{i}_{j = 0} array[j]
                        }
                    } & \\
                %
                %
                %
                =   & \state{
                        & 0 \leq i < length \wedge \\
                        & length = \text{size of array[]} \wedge \\
                        & total = \sum^{i}_{j = 0} array[j]
                    }[i/i'] \wedge \state{
                        i := i + 1
                    }[i/i'] & \\
                %
                %
                %
                =   & \state{
                        & 0 \leq i' < length \wedge \\
                        & length = \text{size of array[]} \wedge \\
                        & total = \sum^{i'}_{j = 0} array[j]
                    } \wedge \state{
                        i = i' + 1
                    } & \\
                %
                %
                %
                =   & \state{
                        & 0 \leq i' < length \wedge \\
                        & length = \text{size of array[]} \wedge \\
                        & total = \sum^{i'}_{j = 0} array[j]
                    } \wedge \state{
                        i - 1 = i'
                    } & \\
                %
                %
                %
                =   & \state{
                        & 0 \leq i-1 < length \wedge \\
                        & length = \text{size of array[]} \wedge \\
                        & total = \sum^{i-1}_{j = 0} array[j]
                    } & \\
                %
                %
                %
                =   & \state{
                        & 0 < i \leq length \wedge \\
                        & length = \text{size of array[]} \wedge \\
                        & total = \sum^{i-1}_{j = 0} array[j]
                    } & \\
                %
                %
                %
                & \Rightarrow \inv &
            \end{flalign*}

            All right, the invariant is correct so we can move on to the next step.
        
        \subsubsection{Proof that $\inv$ is strong enough}
            The next step is to prove that the invariant is true before the loop so we need to prove $\lpre \Rightarrow \inv$.

            \begin{flalign*}
                \lpre = & \state{
                            & 0 \leq length \wedge \\
                            & length = \text{size of array[]} \wedge \\
                            & total = 0 \wedge \\
                            & i = 0
                        } & \\
                %
                %
                %
                    = & \state{
                            & 0 = i \wedge i \leq length \wedge \\
                            & length = \text{size of array[]} \wedge \\
                            & total = \sum^{i-1}_{j = 0} array[j]
                        } & \\
                %
                %
                %
                        & \Rightarrow \inv
            \end{flalign*}

            All right, the invariant is strong enough so we can move on to the next step.

        \subsubsection{Calculate the strongest loop postcondition $\lpost$}
            The last step is to calculate the strongest loop postcondition $\lpost$ so we need to simplify $\state{\inv \wedge \neg \cond}$.

            \begin{flalign*}
                \inv \wedge \neg \cond = & \state{
                    & 0 \leq i \leq length \wedge \\
                    & length = \text{size of array[]} \wedge \\
                    & total = \sum^{i-1}_{j = 0} array[j]
                } \wedge \state{
                    i \geq length
                } & \\
                = & \state{
                    & 0 \leq i \wedge i = length \wedge \\
                    & length = \text{size of array[]} \wedge \\
                    & total = \sum^{i-1}_{j = 0} array[j]
                } & \\
                = & \state{
                    & 0 \leq length \wedge \\
                    & length = \text{size of array[]} \wedge \\
                    & total = \sum^{length-1}_{j = 0} array[j]
                } & \\
                = & \lpost
            \end{flalign*}

    \subsection{The instructions after the loop}
        Finally, we need to calculate the instructions after the loop by doing $\state{\lpost} \term \state{\post}$.

        \begin{flalign*}
                & \ppsp{\term}{\lpost} & \\
            %
            %
            %
            =   & \ppsp{
                    sum := total;
                }{
                    \state{
                        & 0 \leq length \wedge \\
                        & length = \text{size of array[]} \wedge \\
                        & total = \sum^{length-1}_{j = 0} array[j]
                    }
                } & \\
            %
            %
            %
            =   & \state{
                    & 0 \leq length \wedge \\
                    & length = \text{size of array[]} \wedge \\
                    & total = \sum^{length-1}_{j = 0} array[j]
                }[sum/sum']
                \wedge
                \state{
                    sum := total;
                }[sum/sum'] & \\
            %
            %
            %
            =   & \state{
                    & 0 \leq length \wedge \\
                    & length = \text{size of array[]} \wedge \\
                    & total = \sum^{length-1}_{j = 0} array[j]
                } \wedge \state{
                    sum = total
                } & \\
            %
            %
            %
            =   & \state{
                    & 0 \leq length \wedge \\
                    & length = \text{size of array[]} \wedge \\
                    & sum = \sum^{length-1}_{j = 0} array[j]
                } & \\
            %
            %
            %
            & \Rightarrow \post &
        \end{flalign*}

        Everything is proved so the program is correct.
\end{document}